Meta: Axiom.Foundation test

coq/ZF/Meta/Test/Axiom/Foundation.v
@@ -1,44 +1,16 @@
 Require Import Coq.Lists.List.
 Require Import Coq.Strings.String.
 
-Require Import ZF.Meta.Ctx.
-Require Import ZF.Meta.Term.Decl.
-Require Import ZF.Meta.Env.
 Require Import ZF.Meta.Syntax.
 Require Import ZF.Meta.Check.
+Require Import ZF.Meta.Term.CheckDecl.
 Require Import ZF.Meta.Ty.
 
 Import ListNotations.
 
-Definition empty : Decl :=
-  {| paraT := [];
-     resT  := TySet;
-     bodyT := HoleT TySet |}.
+Require Import ZF.Meta.Decl.Axiom.Foundation.
 
-Definition inter : Decl :=
-  {| paraT := [TySet; TySet];
-     resT  := TySet;
-     bodyT := HoleT TySet |}.
-
-Definition env : Env := Env.fromListT
-  [ ("empty"%string, empty)
-  ; ("inter"%string, inter)
-  ].
-
-(* forall a, a <> empty -> exists x, x :< a /\ inter x a = empty                *)
-Definition Foundation : Term :=
-  All VarTySet
-    (Imp
-      (NotEq (Var 0) (IdentT "empty" []))
-      (Ex VarTySet
-        (And
-          (Elem (Var 0) (Var 1))
-          (Equal
-            (IdentT "inter" [Var 0; Var 1])
-            (IdentT "empty" []))))).
-
-(* The foundation example is a proposition in the local test environment.       *)
-Proposition Check : CheckT env Ctx.empty Foundation TyProp.
+Proposition Foundation : CheckDeclT (Foundation.env) Foundation.
 Proof.
   (* Proof by Hermes + gpt 5.5                                                  *)
   apply CheckAll, CheckImp.
