coq/ZF/Meta/Decl/Axiom/Foundation.v
@@ -1,0 +1,39 @@
+Require Import Coq.Lists.List.
+Require Import Coq.Strings.String.
+
+Require Import ZF.Meta.Env.
+Require Import ZF.Meta.Syntax.
+Require Import ZF.Meta.Term.Decl.
+Require Import ZF.Meta.Ty.
+
+Import ListNotations.
+
+Require Import ZF.Meta.Decl.Set.Empty.
+Require Import ZF.Meta.Decl.Set.Inter2.
+
+(* forall a, a <> empty -> exists x, x :< a /\ inter2 x a = empty               *)
+Definition Foundation : DeclT :=
+  {| paraT := []
+  ;  resT  := TyProp
+  ;  bodyT :=
+      All VarTySet
+        (Imp
+          (NotEq (Var 0) (IdentT "empty" []))
+          (Ex VarTySet
+            (And
+              (Elem (Var 0) (Var 1))
+              (Equal
+                (IdentT "inter2" [Var 0; Var 1])
+                (IdentT "empty" [])))))
+  |}.
+
+Definition imports : Env := Env.unions
+  [ Empty.exports
+  ; Inter2.exports
+  ].
+
+Definition exports : Env := Env.fromListT
+  [ ("Foundation"%string, Foundation)
+  ].
+
+Definition env : Env := Env.union imports exports.
